\input{_header}
Développer et réduire les expressions suivantes :
\begin{enumerate}
     \item
     $A=\left(x+2\right)^{2}$
     \item
     $B=\left(5+x\right)\left(5-x\right)$
     \item
     $C=\left(2x-3\right)^{2}$
     \item
     $D=\left(x+2y\right)\left(x-2y\right)$
\end{enumerate}
\begin{corrige}
     \begin{enumerate}
          \item
          On utilise l'identité remarquable $\left(a+b\right)^{2}=a^{2}+2ab+b^{2}$ avec $a=x$ et $b=2$
          \par
          $A=\left(x+2\right)^{2}=x^{2}+2\times x\times 2+2^{2}=x^{2}+4x+4$
          \item
          On utilise l'identité remarquable $\left(a+b\right)\left(a-b\right)=a^{2}-b^{2}$ avec $a=5$ et $b=x$
          \par
          $B=\left(5+x\right)\left(5-x\right)=5^{2}-x^{2}=25-x^{2}$
          \item
          On utilise l'identité remarquable $\left(a-b\right)^{2}=a^{2}-2ab+b^{2}$ avec $a=2x$ et $b=3$
          \par
          C=$\left(2x-3\right)^{2}=\left(2x\right)^{2}-2\times 2x\times 3+3^{2}=4x^{2}-12x+9$
          \item
          On utilise l'identité remarquable $\left(a+b\right)\left(a-b\right)=a^{2}-b^{2}$ avec $a=x$ et $b=2y$
          \par
          $D=\left(x+2y\right)\left(x-2y\right)=x^{2}-\left(2y\right)^{2}=x^{2}-4y^{2}$
     \end{enumerate}
\end{corrige}
\input{_footer}

